Improve parabstr/ws_hub.

theories/parabstr/ws_deques.v
@@ -142,78 +142,25 @@ Section zebre_G.
   Context `{zebre_G : !ZebreG Σ}.
   Context (ws_deques : ws_deques Σ).
 
-  #[local] Definition ws_deques_steal_as_round_aux : val :=
-    rec: "ws_deques_steal_as_round_aux" "t" "sz" "i" "round" "n" :=
+  #[local] Definition ws_deques_steal_as_aux : val :=
+    rec: "ws_deques_steal_as_aux" "t" "sz" "i" "round" "n" :=
       if: "n" ≤ #0 then (
         §None
       ) else (
         let: "j" := ("i" + #1 + random_round_next "round") `rem` "sz" in
         match: ws_deques.(ws_deques_steal_to) "t" "j" with
         | None =>
-            "ws_deques_steal_as_round_aux" "t" "sz" "i" "round" ("n" - #1)
+            "ws_deques_steal_as_aux" "t" "sz" "i" "round" ("n" - #1)
         |_ as "res" =>
             "res"
         end
       ).
-  #[local] Definition ws_deques_steal_as_round : val :=
-    λ: "t" "sz" "i" "round",
-      ws_deques_steal_as_round_aux "t" "sz" "i" "round" ("sz" - #1).
-
-  #[local] Definition ws_deques_try_steal_as_aux : val :=
-    rec: "ws_deques_try_steal_as_aux" "t" "sz" "i" "round" "n" :=
-      if: "n" ≤ #0 then (
-        §None
-      ) else (
-        match: ws_deques_steal_as_round "t" "sz" "i" "round" with
-        | Some <> as "res" =>
-            "res"
-        | None =>
-            Yield ;;
-            random_round_reset "round" ;;
-            "ws_deques_try_steal_as_aux" "t" "sz" "i" "round" ("n" - #1)
-        end
-      ).
-  Definition ws_deques_try_steal_as : val :=
-    λ: "t" "i" "max_round",
-      let: "sz" := ws_deques.(ws_deques_size) "t" in
-      let: "round" := random_round_create ("sz" - #1) in
-      ws_deques_try_steal_as_aux "t" "sz" "i" "round" "max_round".
-
-  #[local] Definition ws_deques_steal_as_aux : val :=
-    rec: "ws_deques_steal_as_aux" "t" "sz" "i" "round" :=
-      match: ws_deques_steal_as_round "t" "sz" "i" "round" with
-      | Some "v" =>
-          "v"
-      | None =>
-          Yield ;;
-          random_round_reset "round" ;;
-          "ws_deques_steal_as_aux" "t" "sz" "i" "round"
-      end.
   Definition ws_deques_steal_as : val :=
-    λ: "t" "i",
+    λ: "t" "i" "round",
       let: "sz" := ws_deques.(ws_deques_size) "t" in
-      let: "round" := random_round_create ("sz" - #1) in
-      ws_deques_steal_as_aux "t" "sz" "i" "round".
+      ws_deques_steal_as_aux "t" "sz" "i" "round" ("sz" - #1).
 
-  Definition ws_deques_pop_try_steal : val :=
-    λ: "t" "i" "max_round",
-      match: ws_deques.(ws_deques_pop) "t" "i" with
-      | Some <> as "res" =>
-          "res"
-      | None =>
-          ws_deques_try_steal_as "t" "i" "max_round"
-      end.
-
-  Definition ws_deques_pop_steal : val :=
-    λ: "t" "i",
-      match: ws_deques.(ws_deques_pop) "t" "i" with
-      | Some "v" =>
-          "v"
-      | None =>
-          ws_deques_steal_as "t" "i"
-      end.
-
-  #[local] Lemma ws_deques_steal_as_round_aux_spec t ι (sz : nat) i round (n : nat) :
+  #[local] Lemma ws_deques_steal_as_aux_spec t ι (sz : nat) i round (n : nat) :
     (0 ≤ i < sz)%Z →
     <<<
       ws_deques.(ws_deques_inv) t ι sz ∗
@@ -221,7 +168,7 @@ Section zebre_G.
     | ∀∀ vss,
       ws_deques.(ws_deques_model) t vss
     >>>
-      ws_deques_steal_as_round_aux t #sz #i round #n @ ↑ι
+      ws_deques_steal_as_aux t #sz #i round #n @ ↑ι
     <<<
       ∃∃ o,
       match o with
@@ -265,7 +212,7 @@ Section zebre_G.
         assert (n - 1 = (n - 1)%nat)%Z as -> by lia.
         wp_apply ("HLöb" with "Hround HΦ").
   Qed.
-  #[local] Lemma ws_deques_steal_as_round_spec t ι (sz : nat) i round :
+  Lemma ws_deques_steal_as_spec t ι (sz : nat) i round :
     (0 ≤ i < sz)%Z →
     <<<
       ws_deques.(ws_deques_inv) t ι sz ∗
@@ -273,7 +220,7 @@ Section zebre_G.
     | ∀∀ vss,
       ws_deques.(ws_deques_model) t vss
     >>>
-      ws_deques_steal_as_round t #sz #i round @ ↑ι
+      ws_deques_steal_as t #i round @ ↑ι
     <<<
       ∃∃ o,
       match o with
@@ -291,219 +238,12 @@ Section zebre_G.
     >>>.
   Proof.
     iIntros "%Hi !> %Φ (#Ht_inv & Hround) HΦ".
-    wp_rec. wp_pures.
+    wp_rec.
+    wp_smart_apply (ws_deques_size_spec with "Ht_inv") as "_".
+    wp_pures.
     assert (sz - 1 = (sz - 1)%nat)%Z as -> by lia.
-    wp_apply (ws_deques_steal_as_round_aux_spec with "[$Ht_inv $Hround] HΦ"); first done.
-  Qed.
-
-  #[local] Lemma ws_deques_try_steal_as_aux_spec t ι (sz : nat) i round n :
-    (0 ≤ i < sz)%Z →
-    (0 ≤ n)%Z →
-    <<<
-      ws_deques.(ws_deques_inv) t ι sz ∗
-      random_round_model' round (sz - 1) (sz - 1)
-    | ∀∀ vss,
-      ws_deques.(ws_deques_model) t vss
-    >>>
-      ws_deques_try_steal_as_aux t #sz #i round #n @ ↑ι
-    <<<
-      ∃∃ o,
-      match o with
-      | None =>
-          ws_deques.(ws_deques_model) t vss
-      | Some v =>
-          ∃ j vs,
-          ⌜Z.to_nat i ≠ j⌝ ∗
-          ⌜vss !! j = Some (v :: vs)⌝ ∗
-          ws_deques.(ws_deques_model) t (<[j := vs]> vss)
-      end
-    | RET o;
-      ∃ n',
-      random_round_model' round (sz - 1) n'
-    >>>.
-  Proof.
-    iIntros "%Hi %Hn !> %Φ (#Ht_inv & Hround) HΦ".
-    iLöb as "HLöb" forall (n Hn).
-    wp_rec. wp_pures.
-    case_bool_decide as Hcase; wp_pures.
-    - iMod "HΦ" as "(%vss & Ht_model & _ & HΦ)".
-      iApply ("HΦ" $! None with "Ht_model [Hround]"); first iSteps.
-    - awp_apply (ws_deques_steal_as_round_spec with "[$Ht_inv $Hround]"); first done.
-      iApply (aacc_aupd with "HΦ"); first done. iIntros "%vss Ht_model".
-      iAaccIntro with "Ht_model"; first iSteps. iIntros ([v |]).
-      + iSteps as (j vs Hj Hlookup) "Ht_model". iExists (Some v). iSteps.
-      + iSteps as (?) "HΦ Hround". iModIntro.
-        wp_smart_apply (random_round_reset_spec' with "Hround") as "Hround".
-        iSteps.
-  Qed.
-  Lemma ws_deques_try_steal_as_spec t ι (sz : nat) i max_round :
-    (0 ≤ i < sz)%Z →
-    (0 ≤ max_round)%Z →
-    <<<
-      ws_deques.(ws_deques_inv) t ι sz
-    | ∀∀ vss,
-      ws_deques.(ws_deques_model) t vss
-    >>>
-      ws_deques_try_steal_as t #i #max_round @ ↑ι
-    <<<
-      ∃∃ o,
-      match o with
-      | None =>
-          ws_deques.(ws_deques_model) t vss
-      | Some v =>
-          ∃ j vs,
-          ⌜Z.to_nat i ≠ j⌝ ∗
-          ⌜vss !! j = Some (v :: vs)⌝ ∗
-          ws_deques.(ws_deques_model) t (<[j := vs]> vss)
-      end
-    | RET o; True
-    >>>.
-  Proof.
-    iIntros "%Hi %Hmax_round !> %Φ #Ht_inv HΦ".
-    wp_rec.
-    wp_smart_apply (ws_deques_size_spec with "Ht_inv") as "_".
-    wp_smart_apply (random_round_create_spec' with "[//]") as (round) "Hround"; first lia.
-    wp_pures.
-    assert (Z.to_nat (sz - 1) = sz - 1) as -> by lia.
-    wp_apply (ws_deques_try_steal_as_aux_spec with "[$Ht_inv $Hround]"); [done.. |].
-    iApply (atomic_update_mono with "[] HΦ").
-    iSteps.
-  Qed.
-
-  #[local] Lemma ws_deques_steal_as_aux_spec t ι (sz : nat) i round :
-    (0 ≤ i < sz)%Z →
-    <<<
-      ws_deques.(ws_deques_inv) t ι sz ∗
-      random_round_model' round (sz - 1) (sz - 1)
-    | ∀∀ vss,
-      ws_deques.(ws_deques_model) t vss
-    >>>
-      ws_deques_steal_as_aux t #sz #i round @ ↑ι
-    <<<
-      ∃∃ j v vs,
-      ⌜Z.to_nat i ≠ j⌝ ∗
-      ⌜vss !! j = Some (v :: vs)⌝ ∗
-      ws_deques.(ws_deques_model) t (<[j := vs]> vss)
-    | RET v;
-      ∃ n',
-      random_round_model' round (sz - 1) n'
-    >>>.
-  Proof.
-    iIntros "%Hi !> %Φ (#Ht_inv & Hround) HΦ".
-    iLöb as "HLöb".
-    wp_rec. wp_pures.
-    awp_apply (ws_deques_steal_as_round_spec with "[$Ht_inv $Hround]"); first done.
-    iApply (aacc_aupd with "HΦ"); first done. iIntros "%vss Ht_model".
-    iAaccIntro with "Ht_model"; first iSteps. iIntros ([v |]); first iSteps.
-    iSteps as (?) "HΦ Hround". iModIntro.
-    wp_smart_apply (random_round_reset_spec' with "Hround") as "Hround".
-    iSteps.
-  Qed.
-  Lemma ws_deques_steal_as_spec t ι (sz : nat) i :
-    (0 ≤ i < sz)%Z →
-    <<<
-      ws_deques.(ws_deques_inv) t ι sz
-    | ∀∀ vss,
-      ws_deques.(ws_deques_model) t vss
-    >>>
-      ws_deques_steal_as t #i @ ↑ι
-    <<<
-      ∃∃ j v vs,
-      ⌜Z.to_nat i ≠ j⌝ ∗
-      ⌜vss !! j = Some (v :: vs)⌝ ∗
-      ws_deques.(ws_deques_model) t (<[j := vs]> vss)
-    | RET v; True
-    >>>.
-  Proof.
-    iIntros "%Hi !> %Φ #Ht_inv HΦ".
-    wp_rec.
-    wp_smart_apply (ws_deques_size_spec with "Ht_inv") as "_".
-    wp_smart_apply (random_round_create_spec' with "[//]") as (round) "Hround"; first lia.
-    wp_pures.
-    assert (Z.to_nat (sz - 1) = sz - 1) as -> by lia.
-    wp_apply (ws_deques_steal_as_aux_spec with "[$Ht_inv $Hround]"); [done.. |].
-    iApply (atomic_update_mono with "[] HΦ").
-    iSteps.
-  Qed.
-
-  Lemma ws_deques_pop_try_steal_spec t ι (sz : nat) i max_round :
-    let i' := Z.to_nat i in
-    (0 ≤ i < sz)%Z →
-    (0 ≤ max_round)%Z →
-    <<<
-      ws_deques.(ws_deques_inv) t ι sz ∗
-      ws_deques.(ws_deques_owner) t i'
-    | ∀∀ vss,
-      ws_deques.(ws_deques_model) t vss
-    >>>
-      ws_deques_pop_try_steal t #i #max_round @ ↑ι
-    <<<
-      ∃∃ o,
-      match o with
-      | None =>
-          ws_deques.(ws_deques_model) t vss
-      | Some v =>
-          ∃ vs,
-            ⌜vss !! i' = Some (vs ++ [v])⌝ ∗
-            ws_deques.(ws_deques_model) t (<[i' := vs]> vss)
-          ∨ ∃ j,
-            ⌜Z.to_nat i ≠ j⌝ ∗
-            ⌜vss !! j = Some (v :: vs)⌝ ∗
-            ws_deques.(ws_deques_model) t (<[j := vs]> vss)
-      end
-    | RET o;
-      ws_deques.(ws_deques_owner) t i'
-    >>>.
-  Proof.
-    iIntros "%i' %Hi %Hmax_round !> %Φ (#Ht_inv & Ht_owner) HΦ".
-    wp_rec.
-    awp_smart_apply (ws_deques_pop_spec with "[$Ht_inv $Ht_owner]"); first lia.
-    iApply (aacc_aupd with "HΦ"); first done. iIntros "%vss Ht_model".
-    iAaccIntro with "Ht_model"; first iSteps. iIntros ([v |]).
-    - iSteps as (vs Hlookup) "Ht_model". iExists (Some v). iSteps.
-    - iStep 6 as (_) "HΦ Ht_owner". iModIntro.
-      awp_apply (ws_deques_try_steal_as_spec with "Ht_inv"); [done.. |].
-      iApply (aacc_aupd_commit with "HΦ"); first done. clear vss. iIntros "%vss Ht_model".
-      iAaccIntro with "Ht_model"; first iSteps. iIntros ([ v |]); iSteps.
-      + iExists (Some v). iSteps.
-      + iExists None. iSteps.
-  Qed.
-
-  Lemma ws_deques_pop_steal_spec t ι (sz : nat) i :
-    let i' := Z.to_nat i in
-    (0 ≤ i < sz)%Z →
-    <<<
-      ws_deques.(ws_deques_inv) t ι sz ∗
-      ws_deques.(ws_deques_owner) t i'
-    | ∀∀ vss,
-      ws_deques.(ws_deques_model) t vss
-    >>>
-      ws_deques_pop_steal t #i @ ↑ι
-    <<<
-      ∃∃ vs v,
-        ⌜vss !! i' = Some (vs ++ [v])⌝ ∗
-        ws_deques.(ws_deques_model) t (<[i' := vs]> vss)
-      ∨ ∃ j,
-        ⌜Z.to_nat i ≠ j⌝ ∗
-        ⌜vss !! j = Some (v :: vs)⌝ ∗
-        ws_deques.(ws_deques_model) t (<[j := vs]> vss)
-    | RET v;
-      ws_deques.(ws_deques_owner) t i'
-    >>>.
-  Proof.
-    iIntros "%i' %Hi !> %Φ (#Ht_inv & Ht_owner) HΦ".
-    wp_rec.
-    awp_smart_apply (ws_deques_pop_spec with "[$Ht_inv $Ht_owner]"); first lia.
-    iApply (aacc_aupd with "HΦ"); first done. iIntros "%vss Ht_model".
-    iAaccIntro with "Ht_model"; first iSteps. iIntros ([v |]); first iSteps.
-    iStep 6 as (_) "HΦ Ht_owner". iModIntro.
-    awp_apply (ws_deques_steal_as_spec with "Ht_inv"); first done.
-    iApply (aacc_aupd_commit with "HΦ"); first done. clear vss. iIntros "%vss Ht_model".
-    iAaccIntro with "Ht_model"; iSteps.
+    wp_apply (ws_deques_steal_as_aux_spec with "[$Ht_inv $Hround] HΦ"); first done.
   Qed.
 End zebre_G.
 
-#[global] Opaque ws_deques_try_steal_as.
 #[global] Opaque ws_deques_steal_as.
-#[global] Opaque ws_deques_pop_try_steal.
-#[global] Opaque ws_deques_pop_steal.
