theories/parabstr/ws_hub.v
@@ -6,13 +6,18 @@ From zebre Require Import
   prelude.
 From zebre.common Require Import
   list.
+From zebre.iris.bi Require Import
+  big_op.
 From zebre.iris.base_logic Require Import
   lib.twins.
 From zebre.language Require Import
   notations
   diaframe.
 From zebre.std Require Import
-  opt.
+  math
+  opt
+  array
+  random_round.
 From zebre.saturn Require Import
   mpmc_queue_1.
 From zebre.parabstr Require Export
@@ -23,21 +28,25 @@ From zebre.parabstr Require Import
 From zebre Require Import
   options.
 
+Implicit Types yield : bool.
 Implicit Types l : location.
 Implicit Types v t : val.
 Implicit Types vs : gmultiset val.
-Implicit Types γ : gname.
 
 #[local] Notation "'deques'" := (
-  in_type "t" 0
+in_type "t" 0
 )(in custom zebre_field
 ).
 #[local] Notation "'foreign'" := (
   in_type "t" 1
 )(in custom zebre_field
 ).
-#[local] Notation "'waiters'" := (
+#[local] Notation "'rounds'" := (
   in_type "t" 2
+)(in custom zebre_field
+).
+#[local] Notation "'waiters'" := (
+  in_type "t" 3
 )(in custom zebre_field
 ).
 
@@ -49,6 +58,7 @@ Section ws_deques.
     λ: "sz",
       { ws_deques.(ws_deques_create) "sz";
         mpmc_queue_create ();
+        array_init "sz" (λ: <>, random_round_create (positive_part ("sz" - #1)));
         waiters_create ()
       }.
 
@@ -67,40 +77,77 @@ Section ws_deques.
       mpmc_queue_push "t".{foreign} "v" ;;
       ws_hub_notify "t".
 
-  #[local] Definition ws_hub_try_steal : val :=
+  Definition ws_hub_pop : val :=
+    λ: "t" "i",
+      ws_deques.(ws_deques_pop) "t".{deques} "i".
+
+  #[local] Definition ws_hub_try_steal_once : val :=
+    λ: "t" "i",
+      let: "round" := array_unsafe_get "t".{rounds} "i" in
+      random_round_reset "round" ;;
+      ws_deques_steal_as ws_deques "t".{deques} "i" "round".
+
+  #[local] Definition ws_hub_try_steal_aux yield : val :=
+    rec: "ws_hub_try_steal_aux" "t" "i" "max_round" :=
+      if: "max_round" ≤ #0 then (
+        §None
+      ) else (
+        match: mpmc_queue_pop "t".{foreign} with
+        | Some <> as "res" =>
+            "res"
+        | None =>
+            match: ws_hub_try_steal_once "t" "i" with
+            | Some <> as "res" =>
+                "res"
+            | None =>
+                (if yield then Yield else ()) ;;
+                "ws_hub_try_steal_aux" "t" "i" ("max_round" - #1)
+            end
+        end
+      ).
+  Definition ws_hub_try_steal : val :=
     λ: "t" "i" "max_round",
-      match: mpmc_queue_pop "t".{foreign} with
+      match: ws_hub_try_steal_aux false "t" "i" "max_round".<0> with
       | Some <> as "res" =>
           "res"
       | None =>
-          ws_deques_try_steal_as ws_deques "t".{deques} "i" "max_round"
+          ws_hub_try_steal_aux true "t" "i" "max_round".<1>
       end.
 
-  #[local] Definition ws_hub_try_pop : val :=
+  Definition ws_hub_pop_try_steal : val :=
     λ: "t" "i" "max_round",
-      match: ws_deques.(ws_deques_pop) "t".{deques} "i" with
+      match: ws_hub_pop "t" "i" with
       | Some <> as "res" =>
           "res"
       | None =>
           ws_hub_try_steal "t" "i" "max_round"
       end.
 
-  Definition ws_hub_pop : val :=
-    rec: "ws_hub_pop" "t" "i" "max_round" :=
-    match: ws_hub_try_pop "t" "i" "max_round" with
+  Definition ws_hub_steal : val :=
+    rec: "ws_hub_steal" "t" "i" "max_round" :=
+      match: ws_hub_try_steal "t" "i" "max_round" with
       | Some "v" =>
           "v"
       | None =>
           let: "waiters" := "t".{waiters} in
           let: "waiter" := waiters_prepare_wait "waiters" in
-          match: ws_hub_try_steal "t" "i" #1 with
+          match: ws_hub_try_steal_once "t" "i" with
           | Some "v" =>
               waiters_cancel_wait "waiters" "waiter" ;;
               "v"
           | None =>
               waiters_commit_wait "waiters" "waiter" ;;
-              "ws_hub_pop" "t" "i" "max_round"
+              "ws_hub_steal" "t" "i" "max_round"
           end
+      end.
+
+  Definition ws_hub_pop_steal : val :=
+    λ: "t" "i" "max_round",
+      match: ws_hub_pop "t" "i" with
+      | Some "v" =>
+          "v"
+      | None =>
+          ws_hub_steal "t" "i" "max_round"
       end.
 End ws_deques.
 
@@ -126,28 +173,69 @@ Section ws_hub_G.
   Context `{ws_hub_G : WsHubG Σ}.
   Context (ws_deques : ws_deques Σ).
 
-  #[local] Definition ws_hub_model₁ γ vs :=
-    twins_twin1 γ (DfracOwn 1) vs.
-  #[local] Definition ws_hub_model₂ γ vs :=
-    twins_twin2 γ vs.
+  Record ws_hub_meta := {
+    ws_hub_meta_size : nat ;
+    ws_hub_meta_deques : val ;
+    ws_hub_meta_foreign : val ;
+    ws_hub_meta_rounds : val ;
+    ws_hub_meta_waiters : val ;
+    ws_hub_meta_model : gname ;
+  }.
+  Implicit Types γ : ws_hub_meta.
 
-  #[local] Definition ws_hub_inv_inner γ deques foreign : iProp Σ :=
+  #[local] Instance ws_hub_meta_eq_dec :
+    EqDecision ws_hub_meta.
+  Proof.
+    solve_decision.
+  Qed.
+  #[local] Instance ws_hub_meta_countable :
+    Countable ws_hub_meta.
+  Proof.
+    pose encode γ := (
+      γ.(ws_hub_meta_size),
+      γ.(ws_hub_meta_deques),
+      γ.(ws_hub_meta_foreign),
+      γ.(ws_hub_meta_rounds),
+      γ.(ws_hub_meta_waiters),
+      γ.(ws_hub_meta_model)
+    ).
+    pose decode := λ '(γ_size, γ_deques, γ_foreign, γ_rounds, γ_waiters, γ_model), {|
+      ws_hub_meta_size := γ_size ;
+      ws_hub_meta_deques := γ_deques ;
+      ws_hub_meta_foreign := γ_foreign ;
+      ws_hub_meta_rounds := γ_rounds ;
+      ws_hub_meta_waiters := γ_waiters ;
+      ws_hub_meta_model := γ_model ;
+    |}.
+    refine (inj_countable' encode decode _). intros []. done.
+  Qed.
+
+  #[local] Definition ws_hub_model₁' γ_model vs :=
+    twins_twin1 γ_model (DfracOwn 1) vs.
+  #[local] Definition ws_hub_model₁ γ vs :=
+    ws_hub_model₁' γ.(ws_hub_meta_model) vs.
+  #[local] Definition ws_hub_model₂' γ_model vs :=
+    twins_twin2 γ_model vs.
+  #[local] Definition ws_hub_model₂ γ vs :=
+    ws_hub_model₂' γ.(ws_hub_meta_model) vs.
+
+  #[local] Definition ws_hub_inv_inner γ : iProp Σ :=
     ∃ vs vss vs_foreign,
     ⌜vs = foldr (λ vs_deques vs, list_to_set_disj vs_deques ⊎ vs) (list_to_set_disj vs_foreign) vss⌝ ∗
-    ws_deques.(ws_deques_model) deques vss ∗
-    mpmc_queue_model foreign vs_foreign ∗
+    ws_deques.(ws_deques_model) γ.(ws_hub_meta_deques) vss ∗
+    mpmc_queue_model γ.(ws_hub_meta_foreign) vs_foreign ∗
     ws_hub_model₂ γ vs.
   Definition ws_hub_inv t ι : iProp Σ :=
-    ∃ l γ deques foreign waiters sz,
+    ∃ l γ,
     ⌜t = #l⌝ ∗
     meta l nroot γ ∗
-    l.[deques] ↦□ deques ∗
-    l.[foreign] ↦□ foreign ∗
-    l.[waiters] ↦□ waiters ∗
-    ws_deques.(ws_deques_inv) deques (ι.@"deques") sz ∗
-    mpmc_queue_inv foreign (ι.@"foreign") ∗
-    waiters_inv waiters ∗
-    inv (ι.@"inv") (ws_hub_inv_inner γ deques foreign).
+    l.[deques] ↦□ γ.(ws_hub_meta_deques) ∗
+    l.[foreign] ↦□ γ.(ws_hub_meta_foreign) ∗
+    l.[waiters] ↦□ γ.(ws_hub_meta_waiters) ∗
+    ws_deques.(ws_deques_inv) γ.(ws_hub_meta_deques) (ι.@"deques") γ.(ws_hub_meta_size) ∗
+    mpmc_queue_inv γ.(ws_hub_meta_foreign) (ι.@"foreign") ∗
+    waiters_inv γ.(ws_hub_meta_waiters) ∗
+    inv (ι.@"inv") (ws_hub_inv_inner γ).
 
   #[using="ws_deques"]
   Definition ws_hub_model t vs : iProp Σ :=
@@ -157,19 +245,17 @@ Section ws_hub_G.
     ws_hub_model₁ γ vs.
 
   Definition ws_hub_owner t i : iProp Σ :=
-    ∃ l γ deques,
+    ∃ l γ round n,
     ⌜t = #l⌝ ∗
     meta l nroot γ ∗
-    l.[deques] ↦□ deques ∗
-    ws_deques.(ws_deques_owner) deques i.
+    l.[deques] ↦□ γ.(ws_hub_meta_deques) ∗
+    l.[rounds] ↦□ γ.(ws_hub_meta_rounds) ∗
+    ws_deques.(ws_deques_owner) γ.(ws_hub_meta_deques) i ∗
+    array_slice γ.(ws_hub_meta_rounds) γ.(ws_hub_meta_size) i DfracDiscarded [round] ∗
+    random_round_model' round (γ.(ws_hub_meta_size) - 1) n.
 
   #[global] Instance ws_hub_model_timeless t vs :
     Timeless (ws_hub_model t vs).
-  Proof.
-    apply _.
-  Qed.
-  #[global] Instance ws_hub_owner_timeless t i :
-    Timeless (ws_hub_owner t i).
   Proof.
     apply _.
   Qed.
@@ -181,9 +267,9 @@ Section ws_hub_G.
 
   #[local] Lemma ws_hub_model_alloc :
     ⊢ |==>
-      ∃ γ,
-      ws_hub_model₁ γ ∅ ∗
-      ws_hub_model₂ γ ∅.
+      ∃ γ_model,
+      ws_hub_model₁' γ_model ∅ ∗
+      ws_hub_model₂' γ_model ∅.
   Proof.
     apply twins_alloc'.
   Qed.
@@ -208,14 +294,13 @@ Section ws_hub_G.
     ws_hub_owner t i -∗
     False.
   Proof.
-    iIntros "(%l & %γ & %deques & -> & _ & #Hl_deques & Howner1) (%_l & %_γ & %_deques & %Heq & _ & _Hl_deques & Howner2)". injection Heq as <-.
+    iIntros "(%l & %γ & %rounds & %n & -> & _ & #Hl_deques & _ & Howner1 & _) (%_l & %_γ & %_rounds & %_n & %Heq & _ & _Hl_deques & _ & Howner2 & _)". injection Heq as <-.
     iDestruct (pointsto_agree with "Hl_deques _Hl_deques") as %<-. iClear "_Hl_deques".
     iApply (ws_deques_owner_exclusive with "Howner1 Howner2").
   Qed.
 
-  Lemma ws_hub_create_spec ι sz (max_round : Z) :
+  Lemma ws_hub_create_spec ι sz :
     (0 ≤ sz)%Z →
-    (0 ≤ max_round)%Z →
     {{{ True }}}
       ws_hub_create ws_deques #sz
     {{{ t,
@@ -226,32 +311,55 @@ Section ws_hub_G.
         ws_hub_owner t i
     }}}.
   Proof.
-    iIntros "%Hsz %Hmax_round %Φ _ HΦ".
+    set sz' := Z.to_nat sz.
+
+    iIntros "%Hsz %Φ _ HΦ".
 
     wp_rec.
 
     wp_smart_apply (ws_deques_create_spec with "[//]") as (deques) "(#Hdeques_inv & Hdeques_model & Hdeques_owner)"; first done.
     wp_apply (mpmc_queue_create_spec with "[//]") as (foreign) "(#Hforeign_inv & Hforeign_model)".
+    wp_smart_apply (array_init_spec_disentangled (λ _ round, random_round_model' round (sz' - 1) (sz' - 1))) as (v_rounds rounds) "(%Hrounds & Hv_rounds & Hrounds)"; first done.
+    { iIntros "!> %i %Hi".
+      wp_smart_apply positive_part_spec.
+      wp_apply (random_round_create_spec' with "[//]"); first lia.
+      rewrite Nat2Z.id. assert (Z.to_nat (sz - 1) = sz' - 1) as -> by lia.
+      iSteps.
+    }
     wp_apply (waiters_create_spec with "[//]") as (waiters) "#Hwaiters_inv".
 
-    wp_record l as "Hmeta" "(Hl_deques & Hl_foreign & Hl_waiters & _)".
+    wp_record l as "Hmeta" "(Hl_deques & Hl_foreign & Hl_rounds & Hl_waiters & _)".
     iMod (pointsto_persist with "Hl_deques") as "#Hl_deques".
     iMod (pointsto_persist with "Hl_foreign") as "#Hl_foreign".
+    iMod (pointsto_persist with "Hl_rounds") as "#Hl_rounds".
     iMod (pointsto_persist with "Hl_waiters") as "#Hl_waiters".
 
-    iMod ws_hub_model_alloc as "(%γ & Hmodel₁ & Hmodel₂)".
+    iMod ws_hub_model_alloc as "(%γ_model & Hmodel₁ & Hmodel₂)".
+
+    pose γ := {|
+      ws_hub_meta_size := sz' ;
+      ws_hub_meta_deques := deques ;
+      ws_hub_meta_foreign := foreign ;
+      ws_hub_meta_rounds := v_rounds ;
+      ws_hub_meta_waiters := waiters ;
+      ws_hub_meta_model := γ_model ;
+    |}.
 
     iMod (meta_set _ _ γ with "Hmeta") as "#Hmeta"; first done.
 
     iApply "HΦ".
-    iSplitR "Hmodel₁ Hdeques_owner".
-    - iSteps.
-      assert (∀ sz, foldr (λ vs_deques vs, list_to_set_disj vs_deques ⊎ vs) ∅ (replicate sz []) = ∅) as ->.
+    iSplitR "Hmodel₁ Hdeques_owner Hv_rounds Hrounds"; iSteps.
+    - assert (∀ sz, foldr (λ vs_deques vs, list_to_set_disj vs_deques ⊎ vs) ∅ (replicate sz []) = ∅) as ->.
       { clear. induction sz as [| sz IH]; first done. rewrite /= left_id //. }
       iSteps.
-    - iSteps.
-      iApply (big_sepL_impl with "Hdeques_owner").
-      iSteps.
+    - iMod (array_model_persist with "Hv_rounds") as "Hv_rounds".
+      iDestruct (array_model_atomize with "Hv_rounds") as "Hv_rounds".
+      iDestruct (big_sepL_sep_2 with "Hv_rounds Hrounds") as "Hrounds".
+      iDestruct (big_sepL_seq_index rounds with "Hdeques_owner") as "Hdeques_owner"; first done.
+      iDestruct (big_sepL_sep_2 with "Hdeques_owner Hrounds") as "H".
+      iApply (big_sepL_seq_index rounds); first done.
+      iApply (big_sepL_impl with "H").
+      rewrite Hrounds. iSteps.
   Qed.
 
   #[local] Lemma ws_hub_notify_spec t ι :
@@ -263,7 +371,7 @@ Section ws_hub_G.
       RET (); True
     }}}.
   Proof.
-    iIntros "%Φ (%l & %γ & %deques & %foreign & %waiters & %sz & -> & #Hmeta & #Hl_deques & #Hl_foreign & #Hl_waiters & #Hdeques_inv & #Hforeign_inv & #Hwaiters_inv & #Hinv) HΦ".
+    iIntros "%Φ (%l & %γ & -> & #Hmeta & #Hl_deques & #Hl_foreign & #Hl_waiters & #Hdeques_inv & #Hforeign_inv & #Hwaiters_inv & #Hinv) HΦ".
 
     wp_rec. wp_load.
     wp_apply (waiters_notify_spec with "Hwaiters_inv HΦ").
@@ -284,13 +392,12 @@ Section ws_hub_G.
       ws_hub_owner t (Z.to_nat i)
     >>>.
   Proof.
-    iIntros "%Hi !> %Φ ((%l & %γ & %deques & %foreign & %waiters & %sz & -> & #Hmeta & #Hl_deques & #Hl_foreign & #Hl_waiters & #Hdeques_inv & #Hforeign_inv & #Hwaiters_inv & #Hinv) & (%_l & %_γ & %_deques & %Heq & _Hmeta & _Hl_deques & Hdeques_owner)) HΦ". injection Heq as <-.
+    iIntros "%Hi !> %Φ ((%l & %γ & -> & #Hmeta & #Hl_deques & #Hl_foreign & #Hl_waiters & #Hdeques_inv & #Hforeign_inv & #Hwaiters_inv & #Hinv) & (%_l & %_γ & %round & %n & %Heq & _Hmeta & _ & #Hl_rounds & Hdeques_owner & #Hv_rounds & Hround)) HΦ". injection Heq as <-.
     iDestruct (meta_agree with "Hmeta _Hmeta") as %<-. iClear "_Hmeta".
-    iDestruct (pointsto_agree with "Hl_deques _Hl_deques") as %<-. iClear "_Hl_deques".
 
     wp_rec. wp_load.
 
-    awp_apply (ws_deques_push_spec with "[$Hdeques_inv $Hdeques_owner]"); first done.
+    awp_apply (ws_deques_push_spec with "[$Hdeques_inv $Hdeques_owner]") without "Hround"; first done.
     iInv "Hinv" as "(%vs & %vss & %vs_foreign & >%Hvs & >Hdeques_model & Hforeign_model & >Hmodel₂)".
     iApply (aacc_aupd_commit with "HΦ"); first solve_ndisj. iIntros "%_vs (%_l & %_γ & %Heq & _Hmeta & Hmodel₁)". injection Heq as <-.
     iDestruct (meta_agree with "Hmeta _Hmeta") as %<-. iClear "_Hmeta".
@@ -310,7 +417,7 @@ Section ws_hub_G.
       { rewrite list_to_set_disj_app. multiset_solver. }
       set_solver.
     }
-    iIntros "Hdeques_owner".
+    iIntros "Hdeques_owner Hround". clear.
 
     wp_smart_apply ws_hub_notify_spec; iSteps.
   Qed.
@@ -327,7 +434,7 @@ Section ws_hub_G.
     | RET (); True
     >>>.
   Proof.
-    iIntros "!> %Φ (%l & %γ & %deques & %foreign & %waiters & %sz & -> & #Hmeta & #Hl_deques & #Hl_foreign & #Hl_waiters & #Hdeques_inv & #Hforeign_inv & #Hwaiters_inv & #Hinv) HΦ".
+    iIntros "!> %Φ (%l & %γ & -> & #Hmeta & #Hl_deques & #Hl_foreign & #Hl_waiters & #Hdeques_inv & #Hforeign_inv & #Hwaiters_inv & #Hinv) HΦ".
 
     wp_rec. wp_load.
 
@@ -349,21 +456,20 @@ Section ws_hub_G.
       rewrite {}Hvs list_to_set_disj_app -foldr_comm_acc_strong; first set_solver by lia.
       f_equal. set_solver by lia.
     }
-    iIntros "_".
+    iIntros "_". clear.
 
     wp_smart_apply ws_hub_notify_spec; iSteps.
   Qed.
 
-  #[local] Lemma ws_hub_try_steal_spec t ι i (max_round : Z) :
+  Lemma ws_hub_pop_spec t ι i :
     (0 ≤ i)%Z →
-    (0 ≤ max_round)%Z →
     <<<
       ws_hub_inv t ι ∗
       ws_hub_owner t (Z.to_nat i)
     | ∀∀ vs,
       ws_hub_model t vs
     >>>
-      ws_hub_try_steal ws_deques t #i #max_round @ ↑ι
+      ws_hub_pop ws_deques t #i @ ↑ι
     <<<
       ∃∃ o,
       match o with
@@ -378,132 +484,26 @@ Section ws_hub_G.
       ws_hub_owner t (Z.to_nat i)
     >>>.
   Proof.
-    iIntros "%Hi %Hmax_round !> %Φ ((%l & %γ & %deques & %foreign & %waiters & %sz & -> & #Hmeta & #Hl_deques & #Hl_foreign & #Hl_waiters & #Hdeques_inv & #Hforeign_inv & #Hwaiters_inv & #Hinv) & (%_l & %_γ & %_deques & %Heq & _Hmeta & _Hl_deques & Hdeques_owner)) HΦ". injection Heq as <-.
+    iIntros "%Hi !> %Φ ((%l & %γ & -> & #Hmeta & #Hl_deques & #Hl_foreign & #Hl_waiters & #Hdeques_inv & #Hforeign_inv & #Hwaiters_inv & #Hinv) & (%_l & %_γ & %round & %n & %Heq & _Hmeta & _ & #Hl_rounds & Hdeques_owner & #Hv_rounds & Hround)) HΦ". injection Heq as <-.
     iDestruct (meta_agree with "Hmeta _Hmeta") as %<-. iClear "_Hmeta".
-    iDestruct (pointsto_agree with "Hl_deques _Hl_deques") as %<-. iClear "_Hl_deques".
 
     wp_rec. wp_load.
 
-    awp_smart_apply (mpmc_queue_pop_spec with "Hforeign_inv").
-    iInv "Hinv" as "(%vs & %vss & %vs_foreign & >%Hvs & Hdeques_model & >Hforeign_model & >Hmodel₂)".
-    iApply (aacc_aupd with "HΦ"); first solve_ndisj. iIntros "%_vs (%_l & %_γ & %Heq & _Hmeta & Hmodel₁)". injection Heq as <-.
-    iDestruct (meta_agree with "Hmeta _Hmeta") as %<-. iClear "_Hmeta".
-    iDestruct (ws_hub_model_agree with "Hmodel₁ Hmodel₂") as %->.
-    iAaccIntro with "Hforeign_model".
-    { iIntros "Hforeign_model !>".
-      iSplitL "Hmodel₁"; first iSteps. iIntros "$ !>".
-      iSplitR "Hdeques_owner"; iSteps.
-    }
-    iIntros "Hforeign_model".
-    destruct vs_foreign as [| v vs_foreign].
-
-    - iLeft. iSplitL "Hmodel₁"; first iSteps. iIntros "!> HΦ !>".
-      iSplitR "Hdeques_owner HΦ"; first iSteps.
-      iIntros "_". clear- Hi Hmax_round.
-
-      wp_load.
-
-      iDestruct (ws_deques_owner_valid with "Hdeques_inv Hdeques_owner") as %?.
-      awp_smart_apply (ws_deques_try_steal_as_spec with "Hdeques_inv"); [lia.. |].
-      iInv "Hinv" as "(%vs & %vss & %vs_foreign & >%Hvs & >Hdeques_model & Hforeign_model & >Hmodel₂)".
-      iApply (aacc_aupd_commit with "HΦ"); first solve_ndisj. iIntros "%_vs (%_l & %_γ & %Heq & _Hmeta & Hmodel₁)". injection Heq as <-.
-      iDestruct (meta_agree with "Hmeta _Hmeta") as %<-. iClear "_Hmeta".
-      iDestruct (ws_hub_model_agree with "Hmodel₁ Hmodel₂") as %->.
-      iAaccIntro with "Hdeques_model".
-      { iIntros "Hdeques_model !>".
-        iSplitL "Hmodel₁"; first iSteps. iIntros "$ !>".
-        iSplitR "Hdeques_owner"; iSteps.
-      }
-      iIntros ([v |]) "Hdeques_model".
-
-      + iDestruct "Hdeques_model" as "(%j & %ws & %Hj & %Hlookup & Hdeques_model)".
-        set vs' := vs ∖ {[+v+]}.
-        iMod (ws_hub_model_update vs' with "Hmodel₁ Hmodel₂") as "(Hmodel₁ & Hmodel₂)".
-        iExists (Some v).
-        iSplitL "Hmodel₁".
-        { iExists vs'. iSteps. iPureIntro.
-          apply gmultiset_disj_union_difference'.
-          rewrite {}Hvs -(take_drop_middle vss j (v :: ws)) // foldr_app /=.
-          rewrite foldr_comm_acc_strong; first multiset_solver.
-          set_solver.
-        }
-        iIntros "!> HΦ !>".
-        iSplitR "Hdeques_owner HΦ".
-        { repeat iExists _. iFrame. iPureIntro.
-          rewrite /vs' Hvs -{1}(take_drop_middle vss j (v :: ws)) // insert_take_drop.
-          { eapply lookup_lt_Some. done. }
-          rewrite !foldr_app /= !foldr_comm_acc_strong; [multiset_solver.. |].
-          multiset_solver.
-        }
-        iSteps.
-
-      + iExists None. iSplitL "Hmodel₁"; first iSteps. iIntros "!> HΦ !>".
-        iSplitR "Hdeques_owner HΦ"; iSteps.
-
-    - set vs' := vs ∖ {[+v+]}.
-      iMod (ws_hub_model_update vs' with "Hmodel₁ Hmodel₂") as "(Hmodel₁ & Hmodel₂)".
-      iRight. iExists (Some v).
-      iSplitL "Hmodel₁".
-      { iExists vs'. iSteps. iPureIntro.
-        apply gmultiset_disj_union_difference'.
-        rewrite {}Hvs foldr_comm_acc_strong; first set_solver by lia.
-        set_solver.
-      }
-      iIntros "!> HΦ !>".
-      iSplitR "Hdeques_owner HΦ".
-      { repeat iExists _. iFrame. iPureIntro.
-        rewrite /vs' Hvs /= foldr_comm_acc_strong; first set_solver by lia.
-        multiset_solver.
-      }
-      iSteps.
-  Qed.
-
-  #[local] Lemma ws_hub_try_pop_spec t ι i max_round :
-    (0 ≤ i)%Z →
-    (0 ≤ max_round)%Z →
-    <<<
-      ws_hub_inv t ι ∗
-      ws_hub_owner t (Z.to_nat i)
-    | ∀∀ vs,
-      ws_hub_model t vs
-    >>>
-      ws_hub_try_pop ws_deques t #i #max_round @ ↑ι
-    <<<
-      ∃∃ o,
-      match o with
-      | None =>
-          ws_hub_model t vs
-      | Some v =>
-          ∃ vs',
-          ⌜vs = {[+v+]} ⊎ vs'⌝ ∗
-          ws_hub_model t vs'
-      end
-    | RET o;
-      ws_hub_owner t (Z.to_nat i)
-    >>>.
-  Proof.
-    iIntros "%Hi %Hmax_round !> %Φ ((%l & %γ & %deques & %foreign & %waiters & %sz & -> & #Hmeta & #Hl_deques & #Hl_foreign & #Hl_waiters & #Hdeques_inv & #Hforeign_inv & #Hwaiters_inv & #Hinv) & (%_l & %_γ & %_deques & %Heq & _Hmeta & _Hl_deques & Hdeques_owner)) HΦ". injection Heq as <-.
-    iDestruct (meta_agree with "Hmeta _Hmeta") as %<-. iClear "_Hmeta".
-    iDestruct (pointsto_agree with "Hl_deques _Hl_deques") as %<-. iClear "_Hl_deques".
-
-    wp_rec. wp_load.
-
-    awp_smart_apply (ws_deques_pop_spec with "[$Hdeques_inv $Hdeques_owner]"); first done.
+    awp_smart_apply (ws_deques_pop_spec with "[$Hdeques_inv $Hdeques_owner]") without "Hround"; first done.
     iInv "Hinv" as "(%vs & %vss & %vs_foreign & >%Hvs & >Hdeques_model & Hforeign_model & >Hmodel₂)".
-    iApply (aacc_aupd with "HΦ"); first solve_ndisj. iIntros "%_vs (%_l & %_γ & %Heq & _Hmeta & Hmodel₁)". injection Heq as <-.
+    iApply (aacc_aupd_commit with "HΦ"); first solve_ndisj. iIntros "%_vs (%_l & %_γ & %Heq & _Hmeta & Hmodel₁)". injection Heq as <-.
     iDestruct (meta_agree with "Hmeta _Hmeta") as %<-. iClear "_Hmeta".
     iDestruct (ws_hub_model_agree with "Hmodel₁ Hmodel₂") as %->.
     iAaccIntro with "Hdeques_model".
     { iIntros "Hdeques_model !>".
-      iSplitL "Hmodel₁"; first iSteps. iIntros "$ !>".
-      iSteps.
+      iSplitL "Hmodel₁"; iSteps.
     }
     iIntros ([v |]) "Hdeques_model".
 
     - iDestruct "Hdeques_model" as "(%ws & %Hlookup & Hdeques_model)".
       set vs' := vs ∖ {[+v+]}.
       iMod (ws_hub_model_update vs' with "Hmodel₁ Hmodel₂") as "(Hmodel₁ & Hmodel₂)".
-      iRight. iExists (Some v).
+      iExists (Some v).
       iSplitL "Hmodel₁".
       { iExists vs'. iSteps. iPureIntro.
         apply gmultiset_disj_union_difference'.
@@ -523,15 +523,79 @@ Section ws_hub_G.
       iSteps.
 
     - iDestruct "Hdeques_model" as "(%Hlookup & Hdeques_model)".
-      iLeft. iSplitL "Hmodel₁"; first iSteps. iIntros "!> HΦ !>".
-      iSplitR "HΦ"; first iSteps.
-      iIntros "Hdeques_owner". clear- Hi Hmax_round.
-
-      wp_smart_apply (ws_hub_try_steal_spec with "[Hdeques_owner] HΦ"); [done.. |].
-      iSteps.
+      iExists None.
+      iSplitL "Hmodel₁"; iSteps.
   Qed.
 
-  Lemma ws_hub_pop_spec t ι i max_round :
+  #[local] Lemma ws_hub_try_steal_once_spec t ι i :
+    (0 ≤ i)%Z →
+    <<<
+      ws_hub_inv t ι ∗
+      ws_hub_owner t (Z.to_nat i)
+    | ∀∀ vs,
+      ws_hub_model t vs
+    >>>
+      ws_hub_try_steal_once ws_deques t #i @ ↑ι
+    <<<
+      ∃∃ o,
+      match o with
+      | None =>
+          ws_hub_model t vs
+      | Some v =>
+          ∃ vs',
+          ⌜vs = {[+v+]} ⊎ vs'⌝ ∗
+          ws_hub_model t vs'
+      end
+    | RET o;
+      ws_hub_owner t (Z.to_nat i)
+    >>>.
+  Proof.
+    iIntros "%Hi !> %Φ ((%l & %γ & -> & #Hmeta & #Hl_deques & #Hl_foreign & #Hl_waiters & #Hdeques_inv & #Hforeign_inv & #Hwaiters_inv & #Hinv) & (%_l & %_γ & %round & %n & %Heq & _Hmeta & _ & #Hl_rounds & Hdeques_owner & #Hv_rounds & Hround)) HΦ". injection Heq as <-.
+    iDestruct (meta_agree with "Hmeta _Hmeta") as %<-. iClear "_Hmeta".
+
+    wp_rec. wp_load.
+    wp_apply (array_unsafe_get_spec_cell with "Hv_rounds") as "_"; first lia.
+    wp_smart_apply (random_round_reset_spec' with "Hround") as "Hround".
+    wp_load.
+
+    iDestruct (ws_deques_owner_valid with "Hdeques_inv Hdeques_owner") as %?.
+    awp_apply (ws_deques_steal_as_spec with "[$Hdeques_inv $Hround]") without "Hdeques_owner"; first lia.
+    iInv "Hinv" as "(%vs & %vss & %vs_foreign & >%Hvs & >Hdeques_model & Hforeign_model & >Hmodel₂)".
+    iApply (aacc_aupd_commit with "HΦ"); first solve_ndisj. iIntros "%_vs (%_l & %_γ & %Heq & _Hmeta & Hmodel₁)". injection Heq as <-.
+    iDestruct (meta_agree with "Hmeta _Hmeta") as %<-. iClear "_Hmeta".
+    iDestruct (ws_hub_model_agree with "Hmodel₁ Hmodel₂") as %->.
+    iAaccIntro with "Hdeques_model".
+    { iIntros "Hdeques_model !>".
+      iSplitL "Hmodel₁"; iSteps.
+    }
+    iIntros ([v |]) "Hdeques_model".
+
+    - iDestruct "Hdeques_model" as "(%j & %ws & %Hj & %Hlookup & Hdeques_model)".
+      set vs' := vs ∖ {[+v+]}.
+      iMod (ws_hub_model_update vs' with "Hmodel₁ Hmodel₂") as "(Hmodel₁ & Hmodel₂)".
+      iExists (Some v).
+      iSplitL "Hmodel₁".
+      { iExists vs'. iSteps. iPureIntro.
+        apply gmultiset_disj_union_difference'.
+        rewrite {}Hvs -(take_drop_middle vss j (v :: ws)) // foldr_app /=.
+        rewrite foldr_comm_acc_strong; first multiset_solver.
+        set_solver.
+      }
+      iIntros "!> HΦ !>".
+      iSplitR "HΦ".
+      { repeat iExists _. iFrame. iPureIntro.
+        rewrite /vs' Hvs -{1}(take_drop_middle vss j (v :: ws)) // insert_take_drop.
+        { eapply lookup_lt_Some. done. }
+        rewrite !foldr_app /= !foldr_comm_acc_strong; [multiset_solver.. |].
+        multiset_solver.
+      }
+      iSteps.
+
+    - iExists None.
+      iSplitL "Hmodel₁"; iSteps.
+  Qed.
+
+  #[local] Lemma ws_hub_try_steal_aux_spec yield t ι i max_round :
     (0 ≤ i)%Z →
     (0 ≤ max_round)%Z →
     <<<
@@ -540,7 +604,189 @@ Section ws_hub_G.
     | ∀∀ vs,
       ws_hub_model t vs
     >>>
-      ws_hub_pop ws_deques t #i #max_round @ ↑ι
+      ws_hub_try_steal_aux ws_deques yield t #i #max_round @ ↑ι
+    <<<
+      ∃∃ o,
+      match o with
+      | None =>
+          ws_hub_model t vs
+      | Some v =>
+          ∃ vs',
+          ⌜vs = {[+v+]} ⊎ vs'⌝ ∗
+          ws_hub_model t vs'
+      end
+    | RET o;
+      ws_hub_owner t (Z.to_nat i)
+    >>>.
+  Proof.
+    intros Hi.
+    iLöb as "HLöb" forall (max_round).
+
+    iIntros "%Hmax_round !> %Φ ((%l & %γ & -> & #Hmeta & #Hl_deques & #Hl_foreign & #Hl_waiters & #Hdeques_inv & #Hforeign_inv & #Hwaiters_inv & #Hinv) & (%_l & %_γ & %round & %n & %Heq & _Hmeta & _ & #Hl_rounds & Hdeques_owner & #Hv_rounds & Hround)) HΦ". injection Heq as <-.
+    iDestruct (meta_agree with "Hmeta _Hmeta") as %<-. iClear "_Hmeta".
+
+    wp_rec. wp_pures.
+    case_bool_decide as Hcase; wp_pures.
+
+    - iMod "HΦ" as "(%vss & Hmodel & _ & HΦ)".
+      iApply ("HΦ" $! None with "Hmodel").
+      iSteps.
+
+    - wp_load.
+
+      awp_smart_apply (mpmc_queue_pop_spec with "Hforeign_inv") without "Hdeques_owner Hround".
+      iInv "Hinv" as "(%vs & %vss & %vs_foreign & >%Hvs & Hdeques_model & >Hforeign_model & >Hmodel₂)".
+      iApply (aacc_aupd with "HΦ"); first solve_ndisj. iIntros "%_vs (%_l & %_γ & %Heq & _Hmeta & Hmodel₁)". injection Heq as <-.
+      iDestruct (meta_agree with "Hmeta _Hmeta") as %<-. iClear "_Hmeta".
+      iDestruct (ws_hub_model_agree with "Hmodel₁ Hmodel₂") as %->.
+      iAaccIntro with "Hforeign_model".
+      { iIntros "Hforeign_model !>".
+        iSplitL "Hmodel₁"; iSteps.
+      }
+      iIntros "Hforeign_model".
+      destruct vs_foreign as [| v vs_foreign].
+
+      + iLeft. iSplitL "Hmodel₁"; first iSteps. iIntros "!> HΦ !>".
+        iSplitR "HΦ"; first iSteps.
+        iIntros "_ (Hdeques_owner & Hround)". clear- Hi Hmax_round Hcase.
+
+        awp_smart_apply (ws_hub_try_steal_once_spec with "[Hdeques_owner Hround]"); [done | iSteps |].
+        iApply (aacc_aupd with "HΦ"); first done. iIntros "%vs Hmodel".
+        iAaccIntro with "Hmodel"; first iSteps. iIntros ([v |]) "Hmodel !>".
+
+        * iRight. iExists (Some v). iFrame.
+          iIntros "HΦ !> Howner". clear.
+
+          iSpecialize ("HΦ" with "Howner").
+          iSteps.
+
+        * iLeft. iFrame.
+          iIntros "HΦ !> Howner". clear- Hi Hmax_round Hcase.
+
+          wp_pures.
+          wp_bind (subst _ _ _).
+          wp_apply (wp_wand _ _ (λ res, ⌜res = ()%V⌝)%I) as (res) "->".
+          { destruct yield; iSteps. }
+          wp_smart_apply ("HLöb" with "[] [$Howner] HΦ"); iSteps.
+
+      + set vs' := vs ∖ {[+v+]}.
+        iMod (ws_hub_model_update vs' with "Hmodel₁ Hmodel₂") as "(Hmodel₁ & Hmodel₂)".
+        iRight. iExists (Some v).
+        iSplitL "Hmodel₁".
+        { iExists vs'. iSteps. iPureIntro.
+          apply gmultiset_disj_union_difference'.
+          rewrite {}Hvs foldr_comm_acc_strong; first set_solver by lia.
+          set_solver.
+        }
+        iIntros "!> HΦ !>".
+        iSplitR "HΦ".
+        { repeat iExists _. iFrame. iPureIntro.
+          rewrite /vs' Hvs /= foldr_comm_acc_strong; first set_solver by lia.
+          multiset_solver.
+        }
+        iSteps.
+  Qed.
+  #[local] Lemma ws_hub_try_steal_spec t ι i max_round_noyield max_round_yield :
+    (0 ≤ i)%Z →
+    (0 ≤ max_round_noyield)%Z →
+    (0 ≤ max_round_yield)%Z →
+    <<<
+      ws_hub_inv t ι ∗
+      ws_hub_owner t (Z.to_nat i)
+    | ∀∀ vs,
+      ws_hub_model t vs
+    >>>
+      ws_hub_try_steal ws_deques t #i (#max_round_noyield, #max_round_yield)%V @ ↑ι
+    <<<
+      ∃∃ o,
+      match o with
+      | None =>
+          ws_hub_model t vs
+      | Some v =>
+          ∃ vs',
+          ⌜vs = {[+v+]} ⊎ vs'⌝ ∗
+          ws_hub_model t vs'
+      end
+    | RET o;
+      ws_hub_owner t (Z.to_nat i)
+    >>>.
+  Proof.
+    iIntros "%Hi %Hmax_round_noyield %Hmax_round_yield !> %Φ (#Hinv & Howner) HΦ".
+
+    wp_rec.
+
+    awp_smart_apply (ws_hub_try_steal_aux_spec with "[$Hinv $Howner]"); [done.. |].
+    iApply (aacc_aupd with "HΦ"); first done. iIntros "%vs Hmodel".
+    iAaccIntro with "Hmodel"; first iSteps. iIntros ([v |]) "Hmodel !>".
+
+    - iRight. iExists (Some v). iFrame.
+      iIntros "HΦ !> Howner". clear.
+
+      iSpecialize ("HΦ" with "Howner").
+      iSteps.
+
+    - iLeft. iFrame.
+      iIntros "HΦ !> Howner". clear- Hi Hmax_round_yield.
+
+      wp_smart_apply (ws_hub_try_steal_aux_spec with "[$Hinv $Howner] HΦ"); done.
+  Qed.
+
+  #[local] Lemma ws_hub_pop_try_steal_spec t ι i max_round_noyield max_round_yield :
+    (0 ≤ i)%Z →
+    (0 ≤ max_round_noyield)%Z →
+    (0 ≤ max_round_yield)%Z →
+    <<<
+      ws_hub_inv t ι ∗
+      ws_hub_owner t (Z.to_nat i)
+    | ∀∀ vs,
+      ws_hub_model t vs
+    >>>
+      ws_hub_pop_try_steal ws_deques t #i (#max_round_noyield, #max_round_yield)%V @ ↑ι
+    <<<
+      ∃∃ o,
+      match o with
+      | None =>
+          ws_hub_model t vs
+      | Some v =>
+          ∃ vs',
+          ⌜vs = {[+v+]} ⊎ vs'⌝ ∗
+          ws_hub_model t vs'
+      end
+    | RET o;
+      ws_hub_owner t (Z.to_nat i)
+    >>>.
+  Proof.
+    iIntros "%Hi %Hmax_round_noyield %Hmax_round_yield !> %Φ (#Hinv & Howner) HΦ".
+
+    wp_rec.
+
+    awp_smart_apply (ws_hub_pop_spec with "[$Hinv $Howner]"); [done.. |].
+    iApply (aacc_aupd with "HΦ"); first done. iIntros "%vs Hmodel".
+    iAaccIntro with "Hmodel"; first iSteps. iIntros ([v |]) "Hmodel !>".
+
+    - iRight. iExists (Some v). iFrame.
+      iIntros "HΦ !> Howner". clear.
+
+      iSpecialize ("HΦ" with "Howner").
+      iSteps.
+
+    - iLeft. iFrame.
+      iIntros "HΦ !> Howner". clear- Hi Hmax_round_noyield Hmax_round_yield.
+
+      wp_smart_apply (ws_hub_try_steal_spec with "[$Hinv $Howner] HΦ"); done.
+  Qed.
+
+  Lemma ws_hub_steal_spec t ι i max_round_noyield max_round_yield :
+    (0 ≤ i)%Z →
+    (0 ≤ max_round_noyield)%Z →
+    (0 ≤ max_round_yield)%Z →
+    <<<
+      ws_hub_inv t ι ∗
+      ws_hub_owner t (Z.to_nat i)
+    | ∀∀ vs,
+      ws_hub_model t vs
+    >>>
+      ws_hub_steal ws_deques t #i (#max_round_noyield, #max_round_yield)%V @ ↑ι
     <<<
       ∃∃ v vs',
       ⌜vs = {[+v+]} ⊎ vs'⌝ ∗
@@ -549,13 +795,13 @@ Section ws_hub_G.
       ws_hub_owner t (Z.to_nat i)
     >>>.
   Proof.
-    iIntros "%Hi %Hmax_round !> %Φ (#Hinv & Howner) HΦ".
+    iIntros "%Hi %Hmax_round_noyield %Hmax_round_yield !> %Φ (#Hinv & Howner) HΦ".
 
     iLöb as "HLöb".
 
     wp_rec.
 
-    awp_smart_apply (ws_hub_try_pop_spec with "[$Hinv $Howner]"); [done.. |].
+    awp_smart_apply (ws_hub_try_steal_spec with "[$Hinv $Howner]"); [done.. |].
     iApply (aacc_aupd with "HΦ"); first done. iIntros "%vs Hmodel".
     iAaccIntro with "Hmodel"; first iSteps. iIntros ([v |]) "Hmodel !>".
 
@@ -565,12 +811,12 @@ Section ws_hub_G.
     - iLeft. iFrame.
       iIntros "HΦ !> Howner". clear- Hi.
 
-      iDestruct "Hinv" as "(%l & %γ & %deques & %foreign & %waiters & %sz & -> & #Hmeta & #Hl_deques & #Hl_foreign & #Hl_waiters & #Hdeques_inv & #Hforeign_inv & #Hwaiters_inv & #Hinv)".
+      iDestruct "Hinv" as "(%l & %γ & -> & #Hmeta & #Hl_deques & #Hl_foreign & #Hl_waiters & #Hdeques_inv & #Hforeign_inv & #Hwaiters_inv & #Hinv)".
 
       wp_load.
       wp_smart_apply (waiters_prepare_wait_spec with "Hwaiters_inv") as (waiter) "Hwaiter".
 
-      awp_smart_apply (ws_hub_try_steal_spec with "[$Howner]") without "Hwaiter"; [done.. | iSteps |].
+      awp_smart_apply (ws_hub_try_steal_once_spec with "[$Howner]") without "Hwaiter"; [done.. | iSteps |].
       iApply (aacc_aupd with "HΦ"); first done. iIntros "%vs Hmodel".
       iAaccIntro with "Hmodel"; first iSteps. iIntros ([v |]) "Hmodel !>".
 
@@ -588,12 +834,56 @@ Section ws_hub_G.
         wp_smart_apply (waiters_commit_wait_spec with "[$Hwaiters_inv $Hwaiter]") as "_".
         wp_smart_apply ("HLöb" with "Howner HΦ").
   Qed.
+
+  Lemma ws_hub_pop_steal_spec t ι i max_round_noyield max_round_yield :
+    (0 ≤ i)%Z →
+    (0 ≤ max_round_noyield)%Z →
+    (0 ≤ max_round_yield)%Z →
+    <<<
+      ws_hub_inv t ι ∗
+      ws_hub_owner t (Z.to_nat i)
+    | ∀∀ vs,
+      ws_hub_model t vs
+    >>>
+      ws_hub_pop_steal ws_deques t #i (#max_round_noyield, #max_round_yield)%V @ ↑ι
+    <<<
+      ∃∃ v vs',
+      ⌜vs = {[+v+]} ⊎ vs'⌝ ∗
+      ws_hub_model t vs'
+    | RET v;
+      ws_hub_owner t (Z.to_nat i)
+    >>>.
+  Proof.
+    iIntros "%Hi %Hmax_round_noyield %Hmax_round_yield !> %Φ (#Hinv & Howner) HΦ".
+
+    wp_rec.
+
+    awp_smart_apply (ws_hub_pop_spec with "[$Hinv $Howner]"); [done.. |].
+    iApply (aacc_aupd with "HΦ"); first done. iIntros "%vs Hmodel".
+    iAaccIntro with "Hmodel"; first iSteps. iIntros ([v |]) "Hmodel !>".
+
+    - iDestruct "Hmodel" as "(%vs' & -> & Hmodel)".
+      iRight. iExists v, vs'. iFrame. iStep.
+      iIntros "HΦ !> Howner". clear.
+
+      iSpecialize ("HΦ" with "Howner").
+      iSteps.
+
+    - iLeft. iFrame.
+      iIntros "HΦ !> Howner". clear- Hi Hmax_round_noyield Hmax_round_yield.
+
+      wp_smart_apply (ws_hub_steal_spec with "[$Hinv $Howner] HΦ"); done.
+  Qed.
 End ws_hub_G.
 
 #[global] Opaque ws_hub_create.
 #[global] Opaque ws_hub_push.
 #[global] Opaque ws_hub_push_foreign.
 #[global] Opaque ws_hub_pop.
+#[global] Opaque ws_hub_try_steal.
+#[global] Opaque ws_hub_pop_try_steal.
+#[global] Opaque ws_hub_steal.
+#[global] Opaque ws_hub_pop_steal.
 
 #[global] Opaque ws_hub_inv.
 #[global] Opaque ws_hub_model.
